Adding some comments and changing notation of contexts

src/main.lean
@@ -27,33 +27,23 @@ inductive Ctx : Type
 | cons : Nat → Typ → Ctx → Ctx 
 
 notation "[]" => Ctx.nil
-notation n":"t"⊹"Γ => Ctx.cons n t Γ 
+notation n":"t","Γ => Ctx.cons n t Γ 
 
 namespace Ctx 
 #check []
-#check 4:base ⊹ []
-#check 4:base ⊹ 3:base ⊹ []
+#check 4:base , []
+#check 4:base , 3:base , []
 
 inductive inCtx : Nat → Ctx → Type 
-| init (Γ : Ctx) (n : Nat) (A : Typ) : inCtx n (n:A ⊹ Γ) 
-| cons (Γ : Ctx) (n n₁ : Nat) (A : Typ) : inCtx n Γ → inCtx n (n₁:A ⊹ Γ)
+| init (Γ : Ctx) (n : Nat) (A : Typ) : inCtx n (n:A , Γ) 
+| cons (Γ : Ctx) (n n₁ : Nat) (A : Typ) : inCtx n Γ → inCtx n (n₁:A , Γ)
 
 notation n"ε"Γ => inCtx n Γ
 notation n"¬ε"Γ => inCtx n Γ → false
 
--- Return a proof that Γ₃ is Γ₁ ++ Γ₂ with no duplicates --
-inductive mergeCtx : Ctx → Ctx → Ctx → Type
-| nil_nil : mergeCtx [] [] []
-| nil_cons : mergeCtx [] Γ Γ 
-| cons_in (n : Nat) (Γ₁ Γ₂ Γ₃ : Ctx) : (n ε Γ₂) → mergeCtx Γ₁ Γ₂ Γ₃ → mergeCtx (n:A ⊹ Γ₁) Γ₂ Γ₃ 
-| cons_out (n : Nat) (Γ₁ Γ₂ Γ₃ : Ctx) : (n ¬ε Γ₂) → mergeCtx Γ₁ Γ₂ Γ₃ → mergeCtx (n:A ⊹ Γ₁) Γ₂ (n:A ⊹ Γ₃) 
-
 inductive validCtx : Ctx → Type 
 | nil : validCtx []
-| cons (n : Nat) (A : Typ) (Γ : Ctx) : (n ¬ε Γ) → validCtx Γ → validCtx (n:A ⊹ Γ)
-notation Γ₃ " ≕ " Γ₁" ⊹ "Γ₂  => mergeCtx Γ₁ Γ₂ Γ₃ 
-
-#check []≕[]⊹[]
+| cons (n : Nat) (A : Typ) (Γ : Ctx) : (n ¬ε Γ) → validCtx Γ → validCtx (n:A , Γ)
 
 inductive Term : Type
 | var : Nat → Term
@@ -70,13 +60,35 @@ namespace Term
 #check (λ(4).$5)($7)
 
 inductive Deduction : Ctx → Term → Typ → Type 
-| var (n : Nat) (A : Typ) : Deduction (n:A ⊹ []) ($ n) A
-| weak (n : Nat) (Γ : Ctx) (A : Typ) : (n ¬ε Γ) → Deduction Γ t A → Deduction (n:B ⊹ Γ) t A 
-| comm (Γ : Ctx) (n₁ n₂ : Nat) (A₁ A₂ : Typ) (t : Term) :
-      Deduction (n₁:A₁ ⊹ n₂:A₂ ⊹ Γ) t A →
-      Deduction (n₂:A₂ ⊹ n₁:A₁ ⊹ Γ) t A
-| abs (n: Nat) (Γ : Ctx) (A B : Typ) : Deduction (n:A ⊹ Γ) ($ n) A → Deduction Γ t B →  Deduction Γ (λ(n).t) (A->B)
-| app (n : Nat) (Γ : Ctx) (t₁ t₂ : Term): Deduction Γ t₁ (A->B) → Deduction Γ t₂ A → Deduction Γ ((t₁)(t₂)) B
+-- n ⊢ n  for any variables --
+| var (n : Nat) (A : Typ) : Deduction (n:A , []) ($ n) A
+
+--     Γ ⊢ t:A 
+    -------------
+--  (n , Γ) ⊢ t:A 
+| weak  (n : Nat) (Γ : Ctx) (A : Typ) 
+        : (n ¬ε Γ) 
+        → Deduction Γ t A 
+        → Deduction (n:B , Γ) t A 
+
+--  n₁ , n₂ , Γ  ⊢ t:A 
+    ------------------
+--  n₂ , n₁ , Γ ⊢ t:A 
+| comm (Γ : Ctx) (n₁ n₂ : Nat) (A₁ A₂ : Typ) (t : Term) 
+        : Deduction (n₁:A₁ , n₂:A₂ , Γ) t A 
+        → Deduction (n₂:A₂ , n₁:A₁ , Γ) t A
+
+--  n + Γ ⊢ n:A  Γ ⊢ t:B 
+    --------------------
+--    Γ ⊢ λ n.t : A->B
+| abs (n: Nat) (Γ : Ctx) (A B : Typ) 
+        : Deduction (n:A , Γ) ($ n) A 
+        → Deduction Γ t B 
+        → Deduction Γ (λ(n).t) (A->B)
+| app (n : Nat) (Γ : Ctx) (t₁ t₂ : Term)
+        : Deduction Γ t₁ (A->B) 
+        → Deduction Γ t₂ A 
+        → Deduction Γ ((t₁)(t₂)) B
 
 -- WARNING, This is "\:" not just ":" --
 notation Γ " ⊢ " t " ∶ " A => Deduction Γ t A 
@@ -87,13 +99,13 @@ theorem invAbs {n : Nat} {Γ : Ctx} {A B : Typ} {t : Term}: (Γ ⊢ λ(x).t ∶ 
     sorry
 
 -- If a weakest context is valid, then a strongest one remains valid --
-theorem weakValidCtx (Γ : Ctx) (n₁ : Nat) (A₁ : Typ) : validCtx (n₁:A₁ ⊹ Γ) → validCtx Γ  := by 
+theorem weakValidCtx (Γ : Ctx) (n₁ : Nat) (A₁ : Typ) : validCtx (n₁:A₁ , Γ) → validCtx Γ  := by 
   intro d 
   cases d 
   case cons A₂ h₁ => assumption
 
 -- Contexts remain valid if we commute their variables ( this should not provable in dependent type theory ! ) --
-theorem commValidCtx {Γ : Ctx} {n₁ n₂ : Nat} {A₁ A₂ : Typ} : validCtx (n₁:A₁ ⊹ n₂:A₂ ⊹ Γ ) → validCtx (n₂:A₂ ⊹ n₁:A₁ ⊹ Γ ) := by
+theorem commValidCtx {Γ : Ctx} {n₁ n₂ : Nat} {A₁ A₂ : Typ} : validCtx (n₁:A₁ , n₂:A₂ , Γ ) → validCtx (n₂:A₂ , n₁:A₁ , Γ ) := by
   intro d 
   apply validCtx.cons 
   . intro d₁ 
@@ -111,7 +123,7 @@ theorem commValidCtx {Γ : Ctx} {n₁ n₂ : Nat} {A₁ A₂ : Typ} : validCtx (
     cases d 
     case a.a.cons h₁ h₂ => 
       apply h₂;apply inCtx.cons;assumption
-    case a.a => exact weakValidCtx Γ n₂ A₂ (weakValidCtx (n₂:A₂ ⊹ Γ) n₁ A₁ d)
+    case a.a => exact weakValidCtx Γ n₂ A₂ (weakValidCtx (n₂:A₂ , Γ) n₁ A₁ d)
     
 -- Prove the soundness of context when a judgment of the form Γ ⊢ x : A is made and x is avariable --
 -- i.e, whenever the judgement is present, the context Γ has to be valid --
@@ -133,7 +145,7 @@ theorem ctxSoundnessVar {n : Nat} {Γ : Ctx} {A : Typ} {t : Term} : (t = $ n ) �
       cases h₃ d₁ 
       case a.cons h₄ h₅ => 
         apply h₅;cases d₃ 
-        case init => exact inCtx.init 
+        case init => exact inCtx.init Γ₁ n₁ B₂ 
         case cons h₆ => 
           cases h₄ 
           case cons h₇ h₈ => have : false = true := h₈ h₆;contradiction 
@@ -170,19 +182,19 @@ theorem ctxNotNilInDeduction {t : Term} {A : Typ} : ([] ⊢ t ∶ A) → False :
     intro d 
   case app => sorry
 
-theorem noDuplicatesInCtx {n : Nat} {A : Typ} {Γ : Ctx} : validCtx (n:A ⊹ Γ) → n ¬ε Γ := by sorry 
+theorem noDuplicatesInCtx {n : Nat} {A : Typ} {Γ : Ctx} : validCtx (n:A , Γ) → n ¬ε Γ := by sorry 
 
 
 
 
-theorem uniqVar {n n' : Nat} {A : Typ} : ((n:A ⊹ []) ⊢ ($ n') ∶ A) → n = n' := by 
+theorem uniqVar {n n' : Nat} {A : Typ} : ((n:A , []) ⊢ ($ n') ∶ A) → n = n' := by 
   intro d  
   cases d 
   case var => rfl
   case weak h d₁ => contradiction 
     
 
-theorem uniqVarInCtx {n n' : Nat} {Γ : Ctx} {t : Term} {A A' B : Typ} : ((n:A ⊹ n':A' ⊹ Γ) ⊢ t ∶ B) → n ≠ n' := by 
+theorem uniqVarInCtx {n n' : Nat} {Γ : Ctx} {t : Term} {A A' B : Typ} : ((n:A , n':A' , Γ) ⊢ t ∶ B) → n ≠ n' := by 
   intro h 
   induction t 
   case var n₁ => 
@@ -194,7 +206,7 @@ theorem uniqVarInCtx {n n' : Nat} {Γ : Ctx} {t : Term} {A A' B : Typ} : ((n:A �
       apply inCtx.init
     case comm h' => 
       intro h₁ 
-      have : validCtx (n':A' ⊹ n:A ⊹ Γ ) := by exact ctxSoundness h' 
+      have : validCtx (n':A' , n:A , Γ ) := by exact ctxSoundness h' 
       rw [h₁] at this 
       cases this 
       case cons hh hhh=> 
@@ -209,8 +221,8 @@ theorem uniqVarInCtx {n n' : Nat} {Γ : Ctx} {t : Term} {A A' B : Typ} : ((n:A �
 
 
 example (n₁ n₂ n₃ n₄ : Nat) (A₁ A₂ A₃ A₄ B: Typ) (t : Term) : 
-  ((n₁:A₁  ⊹ n₂:A₂ ⊹ n₃:A₃  ⊹ n₄:A₄  ⊹ []) ⊢ t ∶ B) 
-  → (n₁:A₁  ⊹ n₃:A₃  ⊹ n₂:A₂  ⊹ n₄:A₄  ⊹ []) ⊢ t ∶ B := by 
+  ((n₁:A₁  , n₂:A₂ , n₃:A₃  , n₄:A₄  , []) ⊢ t ∶ B) 
+  → (n₁:A₁  , n₃:A₃  , n₂:A₂  , n₄:A₄  , []) ⊢ t ∶ B := by 
   intro d
   cases t 
   case var n' => 
@@ -223,7 +235,7 @@ example (n₁ n₂ n₃ n₄ : Nat) (A₁ A₂ A₃ A₄ B: Typ) (t : Term) :
   case app => sorry
 
 
-theorem uniqTypForVar (n : Nat) (A B : Typ ) : ((n:A ⊹ []) ⊢ ($ n) ∶ B)→ A = B := by 
+theorem uniqTypForVar (n : Nat) (A B : Typ ) : ((n:A , []) ⊢ ($ n) ∶ B)→ A = B := by 
   intros d₂
   cases d₂ 
   case var => rfl
@@ -234,16 +246,16 @@ variable (A B : Typ)
 
 --Any term can be constructed no matter the type if we allow free context --
 example {A B : Typ} : Σ Γ : Ctx , Σ t : Term , (Γ ⊢ t ∶ A->B->A) := by
-  let Γ := (0:A->B->A ⊹ [])
+  let Γ := (0:A->B->A , [])
   let t := $0
   have p : Γ ⊢ t ∶ A->B->A := Deduction.var 0 (A->B->A)
   exact ⟨ Γ , ⟨ t , p⟩ ⟩ 
 
 -- The story change if we only allow a restricted context, here we need a more intense derivation --
 
-#check 0:base->base ⊹ 1:base ⊹ []
+#check 0:base->base , 1:base , []
 
-example {A B : Typ} : Σ t : Term , ((0:A->B ⊹ 1:A ⊹ []) ⊢ t ∶ A->B->A) := by
+example {A B : Typ} : Σ t : Term , ((0:A->B , 1:A , []) ⊢ t ∶ A->B->A) := by
   constructor
   case fst => exact λ(1).($0)($1)
   case snd => 
